<?xml version="1.0"?>
<rdf:RDF xmlns="http://www.semanticweb.org/ontologies/knowledge-space#"
     xml:base="http://www.semanticweb.org/ontologies/knowledge-space"
     xmlns:knowledge-space="http://www.semanticweb.org/ontologies/knowledge-space#"
     xmlns:rdf="http://www.w3.org/1999/02/22-rdf-syntax-ns#"
     xmlns:owl="http://www.w3.org/2002/07/owl#"
     xmlns:xml="http://www.w3.org/XML/1998/namespace"
     xmlns:xsd="http://www.w3.org/2001/XMLSchema#"
     xmlns:dcterms="http://purl.org/dc/terms/"
     xmlns:skos="http://www.w3.org/2004/02/skos/core#"
     xmlns:rdfs="http://www.w3.org/2000/01/rdf-schema#"
     xmlns:dc="http://purl.org/dc/elements/1.1/">
    <owl:Ontology rdf:about="http://www.semanticweb.org/ontologies/knowledge-space">
        <rdfs:comment xml:lang="en">Ontology for representing knowledge space</rdfs:comment>
    </owl:Ontology>
    


    <!-- 
    ///////////////////////////////////////////////////////////////////////////////////////
    //
    // Annotation properties
    //
    ///////////////////////////////////////////////////////////////////////////////////////
     -->

    


    <!-- http://purl.org/dc/elements/1.1/creator -->

    <owl:AnnotationProperty rdf:about="http://purl.org/dc/elements/1.1/creator"/>
    


    <!-- http://purl.org/dc/elements/1.1/format -->

    <owl:AnnotationProperty rdf:about="http://purl.org/dc/elements/1.1/format"/>
    


    <!-- http://purl.org/dc/terms/description -->

    <owl:AnnotationProperty rdf:about="http://purl.org/dc/terms/description"/>
    


    <!-- http://purl.org/dc/terms/hasVersion -->

    <owl:AnnotationProperty rdf:about="http://purl.org/dc/terms/hasVersion"/>
    


    <!-- http://purl.org/dc/terms/issued -->

    <owl:AnnotationProperty rdf:about="http://purl.org/dc/terms/issued"/>
    


    <!-- http://purl.org/dc/terms/modified -->

    <owl:AnnotationProperty rdf:about="http://purl.org/dc/terms/modified"/>
    


    <!-- http://purl.org/dc/terms/publisher -->

    <owl:AnnotationProperty rdf:about="http://purl.org/dc/terms/publisher"/>
    


    <!-- http://purl.org/dc/terms/title -->

    <owl:AnnotationProperty rdf:about="http://purl.org/dc/terms/title"/>
    


    <!-- http://www.w3.org/2004/02/skos/core#note -->

    <owl:AnnotationProperty rdf:about="http://www.w3.org/2004/02/skos/core#note"/>
    


    <!-- 
    ///////////////////////////////////////////////////////////////////////////////////////
    //
    // Datatypes
    //
    ///////////////////////////////////////////////////////////////////////////////////////
     -->

    


    <!-- http://www.w3.org/2001/XMLSchema#date -->

    <rdfs:Datatype rdf:about="http://www.w3.org/2001/XMLSchema#date"/>
    


    <!-- 
    ///////////////////////////////////////////////////////////////////////////////////////
    //
    // Object Properties
    //
    ///////////////////////////////////////////////////////////////////////////////////////
     -->

    


    <!-- http://purl.org/dc/terms/source -->

    <owl:ObjectProperty rdf:about="http://purl.org/dc/terms/source"/>
    


    <!-- http://www.semanticweb.org/ontologies/knowledge-space#baseOf -->

    <owl:ObjectProperty rdf:about="http://www.semanticweb.org/ontologies/knowledge-space#baseOf">
        <owl:inverseOf rdf:resource="http://www.semanticweb.org/ontologies/knowledge-space#hasBase"/>
        <rdfs:domain rdf:resource="http://www.semanticweb.org/ontologies/knowledge-space#Data"/>
        <rdfs:range rdf:resource="http://www.semanticweb.org/ontologies/knowledge-space#IITA"/>
        <rdfs:comment xml:lang="en">Data used in IITA methods</rdfs:comment>
        <rdfs:label xml:lang="en">base of</rdfs:label>
    </owl:ObjectProperty>
    


    <!-- http://www.semanticweb.org/ontologies/knowledge-space#baseOfComputation -->

    <owl:ObjectProperty rdf:about="http://www.semanticweb.org/ontologies/knowledge-space#baseOfComputation">
        <owl:inverseOf rdf:resource="http://www.semanticweb.org/ontologies/knowledge-space#computedFrom"/>
        <rdfs:domain rdf:resource="http://www.semanticweb.org/ontologies/knowledge-space#Data"/>
        <rdfs:range rdf:resource="http://www.semanticweb.org/ontologies/knowledge-space#Counterexamples"/>
        <rdfs:comment xml:lang="en">Data used for computation number of counterexamples</rdfs:comment>
        <rdfs:label xml:lang="en">base of computation</rdfs:label>
    </owl:ObjectProperty>
    


    <!-- http://www.semanticweb.org/ontologies/knowledge-space#baseOfGeneration -->

    <owl:ObjectProperty rdf:about="http://www.semanticweb.org/ontologies/knowledge-space#baseOfGeneration">
        <owl:inverseOf rdf:resource="http://www.semanticweb.org/ontologies/knowledge-space#generatedFrom"/>
        <rdfs:domain rdf:resource="http://www.semanticweb.org/ontologies/knowledge-space#Counterexamples"/>
        <rdfs:range rdf:resource="http://www.semanticweb.org/ontologies/knowledge-space#QuasiOrders"/>
        <rdfs:comment xml:lang="en">Counterexamples used for inductively generated list of competing quasi orders</rdfs:comment>
        <rdfs:label xml:lang="en">base of generation</rdfs:label>
    </owl:ObjectProperty>
    


    <!-- http://www.semanticweb.org/ontologies/knowledge-space#computedFrom -->

    <owl:ObjectProperty rdf:about="http://www.semanticweb.org/ontologies/knowledge-space#computedFrom">
        <rdfs:domain rdf:resource="http://www.semanticweb.org/ontologies/knowledge-space#Counterexamples"/>
        <rdfs:range rdf:resource="http://www.semanticweb.org/ontologies/knowledge-space#Data"/>
        <rdfs:comment xml:lang="en">Computed numbers of counterexamples from data</rdfs:comment>
        <rdfs:label xml:lang="en">computed from</rdfs:label>
    </owl:ObjectProperty>
    


    <!-- http://www.semanticweb.org/ontologies/knowledge-space#diagramOf -->

    <owl:ObjectProperty rdf:about="http://www.semanticweb.org/ontologies/knowledge-space#diagramOf">
        <owl:inverseOf rdf:resource="http://www.semanticweb.org/ontologies/knowledge-space#hasDiagram"/>
        <rdfs:domain rdf:resource="http://www.semanticweb.org/ontologies/knowledge-space#HasseDiagram"/>
        <rdfs:range rdf:resource="http://www.semanticweb.org/ontologies/knowledge-space#IITA"/>
        <rdfs:comment xml:lang="en">Hasse diagram of surmise relation</rdfs:comment>
        <rdfs:label xml:lang="en">diagram of</rdfs:label>
    </owl:ObjectProperty>
    


    <!-- http://www.semanticweb.org/ontologies/knowledge-space#generatedFrom -->

    <owl:ObjectProperty rdf:about="http://www.semanticweb.org/ontologies/knowledge-space#generatedFrom">
        <rdfs:domain rdf:resource="http://www.semanticweb.org/ontologies/knowledge-space#QuasiOrders"/>
        <rdfs:range rdf:resource="http://www.semanticweb.org/ontologies/knowledge-space#Counterexamples"/>
        <rdfs:comment xml:lang="en">Inductively generated list of competing quasi orders from the numbers of counterexamples</rdfs:comment>
        <rdfs:label xml:lang="en">generated from</rdfs:label>
    </owl:ObjectProperty>
    


    <!-- http://www.semanticweb.org/ontologies/knowledge-space#hasBase -->

    <owl:ObjectProperty rdf:about="http://www.semanticweb.org/ontologies/knowledge-space#hasBase">
        <rdfs:domain rdf:resource="http://www.semanticweb.org/ontologies/knowledge-space#IITA"/>
        <rdfs:range rdf:resource="http://www.semanticweb.org/ontologies/knowledge-space#Data"/>
        <rdfs:comment xml:lang="en">Refers to the data which are used in IITA methods</rdfs:comment>
        <rdfs:label xml:lang="en">has base</rdfs:label>
    </owl:ObjectProperty>
    


    <!-- http://www.semanticweb.org/ontologies/knowledge-space#hasDiagram -->

    <owl:ObjectProperty rdf:about="http://www.semanticweb.org/ontologies/knowledge-space#hasDiagram">
        <rdfs:domain rdf:resource="http://www.semanticweb.org/ontologies/knowledge-space#IITA"/>
        <rdfs:range rdf:resource="http://www.semanticweb.org/ontologies/knowledge-space#HasseDiagram"/>
        <rdfs:comment xml:lang="en">Hasse diagram of surmise relation</rdfs:comment>
        <rdfs:label xml:lang="en">has diagram</rdfs:label>
    </owl:ObjectProperty>
    


    <!-- http://www.semanticweb.org/ontologies/knowledge-space#hasSelectionSet -->

    <owl:ObjectProperty rdf:about="http://www.semanticweb.org/ontologies/knowledge-space#hasSelectionSet">
        <owl:inverseOf rdf:resource="http://www.semanticweb.org/ontologies/knowledge-space#selectionSetFor"/>
        <rdfs:domain rdf:resource="http://www.semanticweb.org/ontologies/knowledge-space#IITA"/>
        <rdfs:range rdf:resource="http://www.semanticweb.org/ontologies/knowledge-space#QuasiOrders"/>
        <rdfs:comment xml:lang="en">Refers to the list of competing quasi orders used in IITA methods</rdfs:comment>
        <rdfs:label xml:lang="en">has selection set</rdfs:label>
    </owl:ObjectProperty>
    


    <!-- http://www.semanticweb.org/ontologies/knowledge-space#refers -->

    <owl:ObjectProperty rdf:about="http://www.semanticweb.org/ontologies/knowledge-space#refers">
        <rdfs:subPropertyOf rdf:resource="http://purl.org/dc/terms/source"/>
        <rdfs:domain rdf:resource="http://www.semanticweb.org/ontologies/knowledge-space#IITA"/>
        <rdfs:comment xml:lang="en">Refers on scientific document</rdfs:comment>
        <rdfs:label xml:lang="en">refers</rdfs:label>
    </owl:ObjectProperty>
    


    <!-- http://www.semanticweb.org/ontologies/knowledge-space#selectionSetFor -->

    <owl:ObjectProperty rdf:about="http://www.semanticweb.org/ontologies/knowledge-space#selectionSetFor">
        <rdfs:domain rdf:resource="http://www.semanticweb.org/ontologies/knowledge-space#QuasiOrders"/>
        <rdfs:range rdf:resource="http://www.semanticweb.org/ontologies/knowledge-space#IITA"/>
        <rdfs:comment xml:lang="en">Selection set of competing quasi orders used in IITA methods</rdfs:comment>
        <rdfs:label xml:lang="en">selection set for</rdfs:label>
    </owl:ObjectProperty>
    


    <!-- 
    ///////////////////////////////////////////////////////////////////////////////////////
    //
    // Data properties
    //
    ///////////////////////////////////////////////////////////////////////////////////////
     -->

    


    <!-- http://www.semanticweb.org/ontologies/knowledge-space#algorithm -->

    <owl:DatatypeProperty rdf:about="http://www.semanticweb.org/ontologies/knowledge-space#algorithm">
        <rdfs:domain rdf:resource="http://www.semanticweb.org/ontologies/knowledge-space#IITA"/>
        <rdfs:range rdf:resource="http://www.w3.org/2001/XMLSchema#string"/>
        <rdfs:comment xml:lang="en">Name of the used algorithm (e.g. minimized corrected inductive item tree analysis)</rdfs:comment>
        <rdfs:label xml:lang="en">algorithm</rdfs:label>
    </owl:DatatypeProperty>
    


    <!-- http://www.semanticweb.org/ontologies/knowledge-space#diff -->

    <owl:DatatypeProperty rdf:about="http://www.semanticweb.org/ontologies/knowledge-space#diff">
        <rdfs:domain rdf:resource="http://www.semanticweb.org/ontologies/knowledge-space#IITA"/>
        <rdfs:range rdf:resource="http://www.w3.org/2001/XMLSchema#float"/>
        <rdfs:comment xml:lang="en">Fit measure coefficient of selected quasi order</rdfs:comment>
        <rdfs:label xml:lang="en">diff</rdfs:label>
    </owl:DatatypeProperty>
    


    <!-- http://www.semanticweb.org/ontologies/knowledge-space#error -->

    <owl:DatatypeProperty rdf:about="http://www.semanticweb.org/ontologies/knowledge-space#error">
        <rdfs:domain rdf:resource="http://www.semanticweb.org/ontologies/knowledge-space#IITA"/>
        <rdfs:range rdf:resource="http://www.w3.org/2001/XMLSchema#float"/>
        <rdfs:comment xml:lang="en">Error rate</rdfs:comment>
        <rdfs:label xml:lang="en">error</rdfs:label>
    </owl:DatatypeProperty>
    


    <!-- http://www.semanticweb.org/ontologies/knowledge-space#implications -->

    <owl:DatatypeProperty rdf:about="http://www.semanticweb.org/ontologies/knowledge-space#implications">
        <rdfs:domain rdf:resource="http://www.semanticweb.org/ontologies/knowledge-space#IITA"/>
        <rdfs:range rdf:resource="http://www.w3.org/2001/XMLSchema#string"/>
        <rdfs:comment xml:lang="en">List of implications</rdfs:comment>
        <rdfs:label xml:lang="en">implications</rdfs:label>
    </owl:DatatypeProperty>
    


    <!-- http://www.semanticweb.org/ontologies/knowledge-space#labels -->

    <owl:DatatypeProperty rdf:about="http://www.semanticweb.org/ontologies/knowledge-space#labels">
        <rdfs:domain rdf:resource="http://www.semanticweb.org/ontologies/knowledge-space#HasseDiagram"/>
        <rdfs:range rdf:resource="http://www.w3.org/2001/XMLSchema#string"/>
        <rdfs:comment xml:lang="en">Labels used in diagram for representation of items</rdfs:comment>
        <rdfs:label xml:lang="en">labels</rdfs:label>
    </owl:DatatypeProperty>
    


    <!-- http://www.semanticweb.org/ontologies/knowledge-space#length -->

    <owl:DatatypeProperty rdf:about="http://www.semanticweb.org/ontologies/knowledge-space#length">
        <rdfs:domain rdf:resource="http://www.semanticweb.org/ontologies/knowledge-space#QuasiOrders"/>
        <rdfs:range rdf:resource="http://www.w3.org/2001/XMLSchema#nonNegativeInteger"/>
        <rdfs:comment xml:lang="en">Length of list of competing quasi orders</rdfs:comment>
        <rdfs:label xml:lang="en">length</rdfs:label>
    </owl:DatatypeProperty>
    


    <!-- http://www.semanticweb.org/ontologies/knowledge-space#numberOfItems -->

    <owl:DatatypeProperty rdf:about="http://www.semanticweb.org/ontologies/knowledge-space#numberOfItems">
        <rdfs:domain rdf:resource="http://www.semanticweb.org/ontologies/knowledge-space#Data"/>
        <rdfs:range rdf:resource="http://www.w3.org/2001/XMLSchema#nonNegativeInteger"/>
        <rdfs:comment xml:lang="en">Number of items in the dataset</rdfs:comment>
        <rdfs:label xml:lang="en">number of items</rdfs:label>
    </owl:DatatypeProperty>
    


    <!-- http://www.semanticweb.org/ontologies/knowledge-space#numberOfRecords -->

    <owl:DatatypeProperty rdf:about="http://www.semanticweb.org/ontologies/knowledge-space#numberOfRecords">
        <rdfs:domain rdf:resource="http://www.semanticweb.org/ontologies/knowledge-space#Data"/>
        <rdfs:range rdf:resource="http://www.w3.org/2001/XMLSchema#nonNegativeInteger"/>
        <rdfs:comment xml:lang="en">Number of records in the dataset</rdfs:comment>
        <rdfs:label xml:lang="en">number of records</rdfs:label>
    </owl:DatatypeProperty>
    


    <!-- http://www.semanticweb.org/ontologies/knowledge-space#selectionSetIndex -->

    <owl:DatatypeProperty rdf:about="http://www.semanticweb.org/ontologies/knowledge-space#selectionSetIndex">
        <rdfs:domain rdf:resource="http://www.semanticweb.org/ontologies/knowledge-space#IITA"/>
        <rdfs:range rdf:resource="http://www.w3.org/2001/XMLSchema#nonNegativeInteger"/>
        <rdfs:comment xml:lang="en">Index of selected list of implications with best fit measure coefficient</rdfs:comment>
        <rdfs:label xml:lang="en">selection set index</rdfs:label>
    </owl:DatatypeProperty>
    


    <!-- 
    ///////////////////////////////////////////////////////////////////////////////////////
    //
    // Classes
    //
    ///////////////////////////////////////////////////////////////////////////////////////
     -->

    


    <!-- http://www.semanticweb.org/ontologies/knowledge-space#Counterexamples -->

    <owl:Class rdf:about="http://www.semanticweb.org/ontologies/knowledge-space#Counterexamples">
        <rdfs:subClassOf rdf:resource="http://www.w3.org/2002/07/owl#Thing"/>
        <rdfs:comment xml:lang="en">Computed numbers of counterexamples for all items pairs in a dataset</rdfs:comment>
        <rdfs:label xml:lang="en">Counterexamples</rdfs:label>
    </owl:Class>
    


    <!-- http://www.semanticweb.org/ontologies/knowledge-space#Data -->

    <owl:Class rdf:about="http://www.semanticweb.org/ontologies/knowledge-space#Data">
        <rdfs:subClassOf rdf:resource="http://www.w3.org/2002/07/owl#Thing"/>
        <rdfs:comment xml:lang="en">Data resources</rdfs:comment>
        <rdfs:label xml:lang="en">Data</rdfs:label>
    </owl:Class>
    


    <!-- http://www.semanticweb.org/ontologies/knowledge-space#Diagram -->

    <owl:Class rdf:about="http://www.semanticweb.org/ontologies/knowledge-space#Diagram">
        <rdfs:subClassOf rdf:resource="http://www.w3.org/2002/07/owl#Thing"/>
        <rdfs:comment xml:lang="en">Symbolic representation of information</rdfs:comment>
        <rdfs:label xml:lang="en">Diagram</rdfs:label>
    </owl:Class>
    


    <!-- http://www.semanticweb.org/ontologies/knowledge-space#HasseDiagram -->

    <owl:Class rdf:about="http://www.semanticweb.org/ontologies/knowledge-space#HasseDiagram">
        <rdfs:subClassOf rdf:resource="http://www.semanticweb.org/ontologies/knowledge-space#Diagram"/>
        <rdfs:comment xml:lang="en">Hasse diagram of surmise relation</rdfs:comment>
        <rdfs:label xml:lang="en">Hasse Diagram</rdfs:label>
    </owl:Class>
    


    <!-- http://www.semanticweb.org/ontologies/knowledge-space#IITA -->

    <owl:Class rdf:about="http://www.semanticweb.org/ontologies/knowledge-space#IITA">
        <rdfs:subClassOf rdf:resource="http://www.w3.org/2002/07/owl#Thing"/>
        <rdfs:subClassOf>
            <owl:Restriction>
                <owl:onProperty rdf:resource="http://www.semanticweb.org/ontologies/knowledge-space#hasBase"/>
                <owl:someValuesFrom rdf:resource="http://www.semanticweb.org/ontologies/knowledge-space#Data"/>
            </owl:Restriction>
        </rdfs:subClassOf>
        <rdfs:subClassOf>
            <owl:Restriction>
                <owl:onProperty rdf:resource="http://www.semanticweb.org/ontologies/knowledge-space#algorithm"/>
                <owl:qualifiedCardinality rdf:datatype="http://www.w3.org/2001/XMLSchema#nonNegativeInteger">1</owl:qualifiedCardinality>
                <owl:onDataRange rdf:resource="http://www.w3.org/2001/XMLSchema#string"/>
            </owl:Restriction>
        </rdfs:subClassOf>
        <rdfs:subClassOf>
            <owl:Restriction>
                <owl:onProperty rdf:resource="http://www.semanticweb.org/ontologies/knowledge-space#diff"/>
                <owl:qualifiedCardinality rdf:datatype="http://www.w3.org/2001/XMLSchema#nonNegativeInteger">1</owl:qualifiedCardinality>
                <owl:onDataRange rdf:resource="http://www.w3.org/2001/XMLSchema#float"/>
            </owl:Restriction>
        </rdfs:subClassOf>
        <rdfs:subClassOf>
            <owl:Restriction>
                <owl:onProperty rdf:resource="http://www.semanticweb.org/ontologies/knowledge-space#error"/>
                <owl:qualifiedCardinality rdf:datatype="http://www.w3.org/2001/XMLSchema#nonNegativeInteger">1</owl:qualifiedCardinality>
                <owl:onDataRange rdf:resource="http://www.w3.org/2001/XMLSchema#float"/>
            </owl:Restriction>
        </rdfs:subClassOf>
        <rdfs:subClassOf>
            <owl:Restriction>
                <owl:onProperty rdf:resource="http://www.semanticweb.org/ontologies/knowledge-space#implications"/>
                <owl:qualifiedCardinality rdf:datatype="http://www.w3.org/2001/XMLSchema#nonNegativeInteger">1</owl:qualifiedCardinality>
                <owl:onDataRange rdf:resource="http://www.w3.org/2001/XMLSchema#string"/>
            </owl:Restriction>
        </rdfs:subClassOf>
        <rdfs:comment xml:lang="en">Results of performed IITA (Inductive Item Tree Analysis) algorithm</rdfs:comment>
        <rdfs:label xml:lang="en">IITA</rdfs:label>
    </owl:Class>
    


    <!-- http://www.semanticweb.org/ontologies/knowledge-space#QuasiOrders -->

    <owl:Class rdf:about="http://www.semanticweb.org/ontologies/knowledge-space#QuasiOrders">
        <rdfs:subClassOf rdf:resource="http://www.w3.org/2002/07/owl#Thing"/>
        <rdfs:comment xml:lang="en">Inductively generated list of competing quasi orders</rdfs:comment>
        <rdfs:label xml:lang="en">Quasi Orders</rdfs:label>
    </owl:Class>
    


    <!-- 
    ///////////////////////////////////////////////////////////////////////////////////////
    //
    // Annotations
    //
    ///////////////////////////////////////////////////////////////////////////////////////
     -->

    <rdf:Description rdf:about="http://purl.org/dc/elements/1.1/">
        <dcterms:publisher rdf:resource="http://purl.org/dc/aboutdcmi#DCMI"/>
        <dcterms:title xml:lang="en">Dublin Core Metadata Element Set, Version 1.1</dcterms:title>
        <dcterms:modified rdf:datatype="http://www.w3.org/2001/XMLSchema#date">2012-06-14</dcterms:modified>
    </rdf:Description>
    <rdf:Description rdf:about="http://purl.org/dc/elements/1.1/contributor">
        <rdfs:label xml:lang="en">Contributor</rdfs:label>
        <skos:note xml:lang="en">A second property with the same name as this property has been declared in the dcterms: namespace (http://purl.org/dc/terms/).  See the Introduction to the document &quot;DCMI Metadata Terms&quot; (http://dublincore.org/documents/dcmi-terms/) for an explanation.</skos:note>
        <dcterms:hasVersion rdf:resource="http://dublincore.org/usage/terms/history/#contributor-006"/>
        <rdfs:comment xml:lang="en">An entity responsible for making contributions to the resource.</rdfs:comment>
        <dcterms:description xml:lang="en">Examples of a Contributor include a person, an organization, or a service. Typically, the name of a Contributor should be used to indicate the entity.</dcterms:description>
        <dcterms:modified rdf:datatype="http://www.w3.org/2001/XMLSchema#date">2008-01-14</dcterms:modified>
        <dcterms:issued rdf:datatype="http://www.w3.org/2001/XMLSchema#date">1999-07-02</dcterms:issued>
        <rdfs:isDefinedBy rdf:resource="http://purl.org/dc/elements/1.1/"/>
    </rdf:Description>
    <rdf:Description rdf:about="http://purl.org/dc/elements/1.1/coverage">
        <dcterms:hasVersion rdf:resource="http://dublincore.org/usage/terms/history/#coverage-006"/>
        <rdfs:isDefinedBy rdf:resource="http://purl.org/dc/elements/1.1/"/>
        <dcterms:modified rdf:datatype="http://www.w3.org/2001/XMLSchema#date">2008-01-14</dcterms:modified>
        <skos:note xml:lang="en">A second property with the same name as this property has been declared in the dcterms: namespace (http://purl.org/dc/terms/).  See the Introduction to the document &quot;DCMI Metadata Terms&quot; (http://dublincore.org/documents/dcmi-terms/) for an explanation.</skos:note>
        <rdfs:comment xml:lang="en">The spatial or temporal topic of the resource, the spatial applicability of the resource, or the jurisdiction under which the resource is relevant.</rdfs:comment>
        <dcterms:description xml:lang="en">Spatial topic and spatial applicability may be a named place or a location specified by its geographic coordinates. Temporal topic may be a named period, date, or date range. A jurisdiction may be a named administrative entity or a geographic place to which the resource applies. Recommended best practice is to use a controlled vocabulary such as the Thesaurus of Geographic Names [TGN]. Where appropriate, named places or time periods can be used in preference to numeric identifiers such as sets of coordinates or date ranges.</dcterms:description>
        <dcterms:issued rdf:datatype="http://www.w3.org/2001/XMLSchema#date">1999-07-02</dcterms:issued>
        <rdfs:label xml:lang="en">Coverage</rdfs:label>
    </rdf:Description>
    <rdf:Description rdf:about="http://purl.org/dc/elements/1.1/date">
        <dcterms:issued rdf:datatype="http://www.w3.org/2001/XMLSchema#date">1999-07-02</dcterms:issued>
        <skos:note xml:lang="en">A second property with the same name as this property has been declared in the dcterms: namespace (http://purl.org/dc/terms/).  See the Introduction to the document &quot;DCMI Metadata Terms&quot; (http://dublincore.org/documents/dcmi-terms/) for an explanation.</skos:note>
        <dcterms:modified rdf:datatype="http://www.w3.org/2001/XMLSchema#date">2008-01-14</dcterms:modified>
        <rdfs:isDefinedBy rdf:resource="http://purl.org/dc/elements/1.1/"/>
        <dcterms:hasVersion rdf:resource="http://dublincore.org/usage/terms/history/#date-006"/>
        <rdfs:comment xml:lang="en">A point or period of time associated with an event in the lifecycle of the resource.</rdfs:comment>
        <dcterms:description xml:lang="en">Date may be used to express temporal information at any level of granularity.  Recommended best practice is to use an encoding scheme, such as the W3CDTF profile of ISO 8601 [W3CDTF].</dcterms:description>
        <rdfs:label xml:lang="en">Date</rdfs:label>
    </rdf:Description>
    <rdf:Description rdf:about="http://purl.org/dc/elements/1.1/description">
        <dcterms:description xml:lang="en">Description may include but is not limited to: an abstract, a table of contents, a graphical representation, or a free-text account of the resource.</dcterms:description>
        <rdfs:isDefinedBy rdf:resource="http://purl.org/dc/elements/1.1/"/>
        <dcterms:issued rdf:datatype="http://www.w3.org/2001/XMLSchema#date">1999-07-02</dcterms:issued>
        <skos:note xml:lang="en">A second property with the same name as this property has been declared in the dcterms: namespace (http://purl.org/dc/terms/).  See the Introduction to the document &quot;DCMI Metadata Terms&quot; (http://dublincore.org/documents/dcmi-terms/) for an explanation.</skos:note>
        <rdfs:comment xml:lang="en">An account of the resource.</rdfs:comment>
        <dcterms:modified rdf:datatype="http://www.w3.org/2001/XMLSchema#date">2008-01-14</dcterms:modified>
        <rdfs:label xml:lang="en">Description</rdfs:label>
        <dcterms:hasVersion rdf:resource="http://dublincore.org/usage/terms/history/#description-006"/>
    </rdf:Description>
    <rdf:Description rdf:about="http://purl.org/dc/elements/1.1/identifier">
        <dcterms:hasVersion rdf:resource="http://dublincore.org/usage/terms/history/#identifier-006"/>
        <rdfs:isDefinedBy rdf:resource="http://purl.org/dc/elements/1.1/"/>
        <dcterms:description xml:lang="en">Recommended best practice is to identify the resource by means of a string conforming to a formal identification system. </dcterms:description>
        <rdfs:comment xml:lang="en">An unambiguous reference to the resource within a given context.</rdfs:comment>
        <dcterms:issued rdf:datatype="http://www.w3.org/2001/XMLSchema#date">1999-07-02</dcterms:issued>
        <dcterms:modified rdf:datatype="http://www.w3.org/2001/XMLSchema#date">2008-01-14</dcterms:modified>
        <rdfs:label xml:lang="en">Identifier</rdfs:label>
        <skos:note xml:lang="en">A second property with the same name as this property has been declared in the dcterms: namespace (http://purl.org/dc/terms/).  See the Introduction to the document &quot;DCMI Metadata Terms&quot; (http://dublincore.org/documents/dcmi-terms/) for an explanation.</skos:note>
    </rdf:Description>
    <rdf:Description rdf:about="http://purl.org/dc/elements/1.1/language">
        <dcterms:modified rdf:datatype="http://www.w3.org/2001/XMLSchema#date">2008-01-14</dcterms:modified>
        <dcterms:issued rdf:datatype="http://www.w3.org/2001/XMLSchema#date">1999-07-02</dcterms:issued>
        <skos:note xml:lang="en">A second property with the same name as this property has been declared in the dcterms: namespace (http://purl.org/dc/terms/).  See the Introduction to the document &quot;DCMI Metadata Terms&quot; (http://dublincore.org/documents/dcmi-terms/) for an explanation.</skos:note>
        <dcterms:hasVersion rdf:resource="http://dublincore.org/usage/terms/history/#language-007"/>
        <rdfs:label xml:lang="en">Language</rdfs:label>
        <dcterms:description xml:lang="en">Recommended best practice is to use a controlled vocabulary such as RFC 4646 [RFC4646].</dcterms:description>
        <rdfs:isDefinedBy rdf:resource="http://purl.org/dc/elements/1.1/"/>
        <rdfs:comment xml:lang="en">A language of the resource.</rdfs:comment>
        <rdfs:seeAlso rdf:resource="http://www.ietf.org/rfc/rfc4646.txt"/>
    </rdf:Description>
    <rdf:Description rdf:about="http://purl.org/dc/elements/1.1/publisher">
        <skos:note xml:lang="en">A second property with the same name as this property has been declared in the dcterms: namespace (http://purl.org/dc/terms/).  See the Introduction to the document &quot;DCMI Metadata Terms&quot; (http://dublincore.org/documents/dcmi-terms/) for an explanation.</skos:note>
        <dcterms:hasVersion rdf:resource="http://dublincore.org/usage/terms/history/#publisher-006"/>
        <dcterms:issued rdf:datatype="http://www.w3.org/2001/XMLSchema#date">1999-07-02</dcterms:issued>
        <dcterms:modified rdf:datatype="http://www.w3.org/2001/XMLSchema#date">2008-01-14</dcterms:modified>
        <rdfs:label xml:lang="en">Publisher</rdfs:label>
        <rdfs:isDefinedBy rdf:resource="http://purl.org/dc/elements/1.1/"/>
        <dcterms:description xml:lang="en">Examples of a Publisher include a person, an organization, or a service. Typically, the name of a Publisher should be used to indicate the entity.</dcterms:description>
        <rdfs:comment xml:lang="en">An entity responsible for making the resource available.</rdfs:comment>
    </rdf:Description>
    <rdf:Description rdf:about="http://purl.org/dc/elements/1.1/relation">
        <dcterms:hasVersion rdf:resource="http://dublincore.org/usage/terms/history/#relation-006"/>
        <dcterms:description xml:lang="en">Recommended best practice is to identify the related resource by means of a string conforming to a formal identification system. </dcterms:description>
        <rdfs:label xml:lang="en">Relation</rdfs:label>
        <dcterms:modified rdf:datatype="http://www.w3.org/2001/XMLSchema#date">2008-01-14</dcterms:modified>
        <dcterms:issued rdf:datatype="http://www.w3.org/2001/XMLSchema#date">1999-07-02</dcterms:issued>
        <skos:note xml:lang="en">A second property with the same name as this property has been declared in the dcterms: namespace (http://purl.org/dc/terms/).  See the Introduction to the document &quot;DCMI Metadata Terms&quot; (http://dublincore.org/documents/dcmi-terms/) for an explanation.</skos:note>
        <rdfs:comment xml:lang="en">A related resource.</rdfs:comment>
        <rdfs:isDefinedBy rdf:resource="http://purl.org/dc/elements/1.1/"/>
    </rdf:Description>
    <rdf:Description rdf:about="http://purl.org/dc/elements/1.1/rights">
        <dcterms:hasVersion rdf:resource="http://dublincore.org/usage/terms/history/#rights-006"/>
        <rdfs:isDefinedBy rdf:resource="http://purl.org/dc/elements/1.1/"/>
        <skos:note xml:lang="en">A second property with the same name as this property has been declared in the dcterms: namespace (http://purl.org/dc/terms/).  See the Introduction to the document &quot;DCMI Metadata Terms&quot; (http://dublincore.org/documents/dcmi-terms/) for an explanation.</skos:note>
        <dcterms:issued rdf:datatype="http://www.w3.org/2001/XMLSchema#date">1999-07-02</dcterms:issued>
        <dcterms:description xml:lang="en">Typically, rights information includes a statement about various property rights associated with the resource, including intellectual property rights.</dcterms:description>
        <rdfs:label xml:lang="en">Rights</rdfs:label>
        <dcterms:modified rdf:datatype="http://www.w3.org/2001/XMLSchema#date">2008-01-14</dcterms:modified>
        <rdfs:comment xml:lang="en">Information about rights held in and over the resource.</rdfs:comment>
    </rdf:Description>
    <rdf:Description rdf:about="http://purl.org/dc/elements/1.1/source">
        <dcterms:hasVersion rdf:resource="http://dublincore.org/usage/terms/history/#source-006"/>
        <skos:note xml:lang="en">A second property with the same name as this property has been declared in the dcterms: namespace (http://purl.org/dc/terms/).  See the Introduction to the document &quot;DCMI Metadata Terms&quot; (http://dublincore.org/documents/dcmi-terms/) for an explanation.</skos:note>
        <rdfs:isDefinedBy rdf:resource="http://purl.org/dc/elements/1.1/"/>
        <rdfs:comment xml:lang="en">A related resource from which the described resource is derived.</rdfs:comment>
        <dcterms:modified rdf:datatype="http://www.w3.org/2001/XMLSchema#date">2008-01-14</dcterms:modified>
        <dcterms:issued rdf:datatype="http://www.w3.org/2001/XMLSchema#date">1999-07-02</dcterms:issued>
        <dcterms:description xml:lang="en">The described resource may be derived from the related resource in whole or in part. Recommended best practice is to identify the related resource by means of a string conforming to a formal identification system.</dcterms:description>
        <rdfs:label xml:lang="en">Source</rdfs:label>
    </rdf:Description>
    <rdf:Description rdf:about="http://purl.org/dc/elements/1.1/subject">
        <dcterms:description xml:lang="en">Typically, the subject will be represented using keywords, key phrases, or classification codes. Recommended best practice is to use a controlled vocabulary.</dcterms:description>
        <skos:note xml:lang="en">A second property with the same name as this property has been declared in the dcterms: namespace (http://purl.org/dc/terms/).  See the Introduction to the document &quot;DCMI Metadata Terms&quot; (http://dublincore.org/documents/dcmi-terms/) for an explanation.</skos:note>
        <dcterms:issued rdf:datatype="http://www.w3.org/2001/XMLSchema#date">1999-07-02</dcterms:issued>
        <rdfs:label xml:lang="en">Subject</rdfs:label>
        <rdfs:comment xml:lang="en">The topic of the resource.</rdfs:comment>
        <rdfs:isDefinedBy rdf:resource="http://purl.org/dc/elements/1.1/"/>
        <dcterms:modified rdf:datatype="http://www.w3.org/2001/XMLSchema#date">2012-06-14</dcterms:modified>
        <dcterms:hasVersion rdf:resource="http://dublincore.org/usage/terms/history/#subject-007"/>
    </rdf:Description>
    <rdf:Description rdf:about="http://purl.org/dc/elements/1.1/title">
        <dcterms:modified rdf:datatype="http://www.w3.org/2001/XMLSchema#date">2008-01-14</dcterms:modified>
        <rdfs:comment xml:lang="en">A name given to the resource.</rdfs:comment>
        <skos:note xml:lang="en">A second property with the same name as this property has been declared in the dcterms: namespace (http://purl.org/dc/terms/).  See the Introduction to the document &quot;DCMI Metadata Terms&quot; (http://dublincore.org/documents/dcmi-terms/) for an explanation.</skos:note>
        <rdfs:label xml:lang="en">Title</rdfs:label>
        <dcterms:issued rdf:datatype="http://www.w3.org/2001/XMLSchema#date">1999-07-02</dcterms:issued>
        <dcterms:hasVersion rdf:resource="http://dublincore.org/usage/terms/history/#title-006"/>
        <rdfs:isDefinedBy rdf:resource="http://purl.org/dc/elements/1.1/"/>
    </rdf:Description>
    <rdf:Description rdf:about="http://purl.org/dc/elements/1.1/type">
        <dcterms:hasVersion rdf:resource="http://dublincore.org/usage/terms/history/#type-006"/>
        <rdfs:comment xml:lang="en">The nature or genre of the resource.</rdfs:comment>
        <rdfs:label xml:lang="en">Type</rdfs:label>
        <rdfs:isDefinedBy rdf:resource="http://purl.org/dc/elements/1.1/"/>
        <dcterms:description xml:lang="en">Recommended best practice is to use a controlled vocabulary such as the DCMI Type Vocabulary [DCMITYPE]. To describe the file format, physical medium, or dimensions of the resource, use the Format element.</dcterms:description>
        <dcterms:issued rdf:datatype="http://www.w3.org/2001/XMLSchema#date">1999-07-02</dcterms:issued>
        <skos:note xml:lang="en">A second property with the same name as this property has been declared in the dcterms: namespace (http://purl.org/dc/terms/).  See the Introduction to the document &quot;DCMI Metadata Terms&quot; (http://dublincore.org/documents/dcmi-terms/) for an explanation.</skos:note>
        <dcterms:modified rdf:datatype="http://www.w3.org/2001/XMLSchema#date">2008-01-14</dcterms:modified>
    </rdf:Description>
    


    <!-- 
    ///////////////////////////////////////////////////////////////////////////////////////
    //
    // General axioms
    //
    ///////////////////////////////////////////////////////////////////////////////////////
     -->

    <rdf:Description>
        <rdf:type rdf:resource="http://www.w3.org/2002/07/owl#AllDisjointClasses"/>
        <owl:members rdf:parseType="Collection">
            <rdf:Description rdf:about="http://www.semanticweb.org/ontologies/knowledge-space#Counterexamples"/>
            <rdf:Description rdf:about="http://www.semanticweb.org/ontologies/knowledge-space#Data"/>
            <rdf:Description rdf:about="http://www.semanticweb.org/ontologies/knowledge-space#Diagram"/>
            <rdf:Description rdf:about="http://www.semanticweb.org/ontologies/knowledge-space#IITA"/>
            <rdf:Description rdf:about="http://www.semanticweb.org/ontologies/knowledge-space#QuasiOrders"/>
        </owl:members>
    </rdf:Description>
</rdf:RDF>



<!-- Generated by the OWL API (version 4.2.6.20160910-2108) https://github.com/owlcs/owlapi -->

